Reorganized pipeline NOC into modules

noc/Router.v
@@ -1,249 +1,126 @@
+Require Import Types.
 Require Import Koika.Frontend.
 Require Import Koika.Std.
 Require Import Koika.Testing.
 
+Module Type Registers.
+Parameter reg_t : Type.
+End Registers.
 
-(* Structure of standard flit *)
-(* also used as burst header *)
-(* HW-Doc.pdf page 8 *)
+Module Router (Regs:Registers).
+Import Regs.
+Import Types.
+Definition r_send (reg_name: reg_t) : UInternalFunction reg_t empty_ext_fn_t :=
+  {{ fun r_send (value: bits_t sz) : unit_t =>
+    write0(reg_name, value)
+  }}.
 
-Module Types.
+Definition r_receive (reg_name: reg_t) : UInternalFunction reg_t empty_ext_fn_t :=
+  {{ fun r_receive () : bits_t sz =>
+    read0(reg_name)
+  }}.
 
-  Definition xy_cord :=
-    {|
-    struct_name := "xy_cord";
-    struct_fields :=
-      [
-        ("x" , bits_t 1);
-        ("y" , bits_t 1)
-      ]
-    |}.
+Definition _routestart_r (r_addr2: nat) (r0_send r0_receive: UInternalFunction reg_t empty_ext_fn_t) 
+: uaction reg_t empty_ext_fn_t :=
+UBind "r_addr" (USugar (UConstBits (Bits.of_nat 4 r_addr2)))
+{{
+    let m0 := r0_receive() in (*router input policy will be added here*)
+    let msg := unpack(struct_t basic_flit, m0) in
+    let new_data := get(msg, new) in
+    let src_p := get(msg, src) in
+    (( if (src_p != r_addr && new_data) then 
+        let trg_x := get(msg, trg_x) in
+        let trg_y := get(msg, trg_y) in
+        let src_x := get(unpack(struct_t router_address, r_addr), x) in
+        let src_y := get(unpack(struct_t router_address, r_addr), y) in
+        (*r_addr[|2`d0| :+ 2] if not using struct*)
+        if trg_x > src_x then
+        r0_send(pack(subst(msg, src, r_addr)))
+        else if trg_x < src_x then
+        fail
+        else
+        pass    (*Pass to tile from this block*)
+    else
+    pass ))
+}}.
   
-  Definition standard_flit :=
-  {|
-  struct_name := "standard_flit";
-  struct_fields :=
-    [
-      (* if this flit starts burst - if it is a burst header *)
-      ("burst"     , bits_t 1 );
-      (* if this flit expects and acknowledgement *)
-      ("arq"       , bits_t 1 );
-      (* byte selector of payload *)
-      (*
-      header flit only: specifies the first [3:0] and last [7:4]
-      valid byte of the data in the payload flits
-      *)
-      ("bsel"      , bits_t 8 );
-      ("src_modid" , bits_t 8 ); 
-      ("src_chipid", bits_t 6 );
-      ("trg_modid" , bits_t 8 );
-      ("trg_chipid", bits_t 6 );
-      (* read, write .. etc *)
-      ("mode"      , bits_t 4 );
-      (* destination address *)
-      ("addr"      , bits_t 32);
-      (* header flit only: number of upcomming payload flits *)
-      ("data"      , bits_t 64)
-    ]
-  |}.
-
-  Definition basic_flit :=
-  {|
-  struct_name := "basic_flit";
-  struct_fields :=
-    [
-      ("trg" , bits_t 2);
-      ("data" , bits_t 4)
-    ]
-  |}.
-
-End Types.
-
-Module Design.
-
-  Import Types.
-
-  Notation sz := 6.
-
-  Inductive reg_t :=
-      | in0
-      | in1
-      | in0nd
-      | in1nd
-      | ou0
-      | ou1
-      .
-
-(*  Inductive ext_fn_t :=
-    | Inputin0
-    | Inputin1
-      .
-*)
-
-Definition send1: UInternalFunction reg_t empty_ext_fn_t :=
-  {{ fun send1 (value: bits_t 6) : unit_t =>
-    write0(ou1, value)
-  }}.
-
-Definition receive1: UInternalFunction reg_t empty_ext_fn_t :=
-  {{ fun receive1 () : bits_t 6 =>
-    read0(in1)
-  }}.
-
-Definition send0: UInternalFunction reg_t empty_ext_fn_t :=
-  {{ fun send0 (value: bits_t 6) : unit_t =>
-    write0(ou0, value)
-  }}.
-
-Definition receive0: UInternalFunction reg_t empty_ext_fn_t :=
-  {{ fun receive0 () : bits_t 6 =>
-    read0(in0)
-  }}.
-
-
-Definition R reg :=
-  match reg with
-  | in0 => bits_t (struct_sz basic_flit)
-  | in1 => bits_t (struct_sz basic_flit)
-  | in0nd => bits_t 1
-  | in1nd => bits_t 1
-  | ou0 => bits_t (struct_sz basic_flit)
-  | ou1 => bits_t (struct_sz basic_flit)
-  end.
-
-Definition r idx : R idx :=
-  match idx with
-  | in0 => Bits.of_nat 6 49
-  | in1 => Bits.of_nat 6 20
-  | in0nd => Bits.of_nat 1 1
-  | in1nd => Bits.of_nat 1 1
-  | ou0 => Bits.zero
-  | ou1 => Bits.zero
-  end.
-
-Inductive rule_name_t :=
-  | route0_r
-  | route1_r.
-
-Definition _route0_r i i_nd : uaction reg_t empty_ext_fn_t :=
+Definition _routecenter_r (r_addr2: nat) (r0_send r1_send r0_receive r1_receive: UInternalFunction reg_t empty_ext_fn_t) 
+: uaction reg_t empty_ext_fn_t :=
+  UBind "r_addr" (USugar (UConstBits (Bits.of_nat 4 r_addr2)))
   {{
-    let newdata := read0(i_nd) in
-    write0(i_nd, Ob~0);
-  if newdata then
-    let m0 := read0(i) in
-    let addr0 := get(unpack(struct_t basic_flit, m0), trg) in
-    if !addr0 then
-        write0(ou0, m0)
-    else 
-      write0(ou1, m0)
+  let m0 := r0_receive() in (*router input policy will be added here*)
+  let m1 := r1_receive() in 
+  let msg := unpack(struct_t basic_flit, m0) in
+  let new_data := get(msg, new) in
+  let src_p := get(msg, src) in
+  (( if (src_p != r_addr && new_data) then
+      r0_send(pack(subst(msg, new, Ob~0)));
+      let trg_x := get(msg, trg_x) in
+      let trg_y := get(msg, trg_y) in
+      let src_x := get(unpack(struct_t router_address, r_addr), x) in
+      let src_y := get(unpack(struct_t router_address, r_addr), y) in
+      (*r_addr[|2`d0| :+ 2] if not using struct*)
+      if trg_x > src_x then
+      r1_send(pack(subst(msg, src, r_addr)))
+      else if trg_x < src_x then
+      r0_send(pack(subst(msg, src, r_addr)))
+      else
+      pass    (*Pass to tile from this block*)
   else
-    fail
-    (*write0(ou0, Ob~0~0~0~0~0)*) 
+  pass ));
+  let msg1 := unpack(struct_t basic_flit, m1) in
+  let new_data := get(msg1, new) in
+  let src_p := get(msg1, src) in
+  (( if (src_p != r_addr && new_data) then
+      r1_send(pack(subst(msg1, new, Ob~0)));
+      let trg_x := get(msg1, trg_x) in
+      let trg_y := get(msg1, trg_y) in
+      let src_x := get(unpack(struct_t router_address, r_addr), x) in
+      let src_y := get(unpack(struct_t router_address, r_addr), y) in
+      (*r_addr[|2`d0| :+ 2] if not using struct*)
+      if trg_x > src_x then
+      r1_send(pack(subst(msg1, src, r_addr)))
+      else if trg_x < src_x then
+      r0_send(pack(subst(msg1, src, r_addr)))
+      else
+      pass    (*Pass to tile from this block*)
+  else
+  pass ))
+
   }}.
 
-
-Definition _routexy_r i : uaction reg_t empty_ext_fn_t :=
+Definition _routeend_r (r_addr2: nat) (r0_send r0_receive: UInternalFunction reg_t empty_ext_fn_t) 
+: uaction reg_t empty_ext_fn_t :=
+  UBind "r_addr" (USugar (UConstBits (Bits.of_nat 4 r_addr2)))
   {{
-    let r_addr := Ob~0~0 in
-    let m0 := read0(i) in
-    let addr := get(unpack(struct_t basic_flit, m0), trg) in
-    if addr[Ob~1] > r_addr[Ob~1] then
-        write0(ou0, m0)
-    else if addr[Ob~0] > r_addr[Ob~0] then
-        write0(ou1, m0)
-    else
-      pass
+  let m0 := r0_receive() in (*router input policy will be added here*)
+  let msg := unpack(struct_t basic_flit, m0) in
+  let new_data := get(msg, new) in
+  let src_p := get(msg, src) in
+  (( if (src_p != r_addr && new_data) then 
+      let trg_x := get(msg, trg_x) in
+      let trg_y := get(msg, trg_y) in
+      let src_x := get(unpack(struct_t router_address, r_addr), x) in
+      let src_y := get(unpack(struct_t router_address, r_addr), y) in
+      (*r_addr[|2`d0| :+ 2] if not using struct*)
+      if trg_x > src_x then
+      fail
+      else if trg_x < src_x then
+      r0_send(pack(subst(msg, src, r_addr)))
+      else
+      pass    (*Pass to tile from this block*)
+  else
+  pass ))
   }}.
 
-Check Ob~0~0.
-Compute {{Ob~0~0[Ob~0]}}.
-Print Syntax.uaction. 
-Definition _routepr_r (r_addr2: bits_t 2) (receive send0 send1: UInternalFunction reg_t empty_ext_fn_t) : uaction reg_t empty_ext_fn_t :=
-  UBind "r_addr" (USugar (UConstBits r_addr2))
-  {{
-      let m0 := receive() in
-       let addr := get(unpack(struct_t basic_flit, m0), trg) in
-    if addr[Ob~1] > r_addr[Ob~1] then
-        send0(m0)
-    else if addr[Ob~0] > r_addr[Ob~0] then
-        send1(m0)
-    else
-      pass
-  }}.
+Definition routecenterfn (n:nat) (r1 r2 : reg_t): uaction reg_t empty_ext_fn_t :=
+  _routecenter_r n (r_send r1) (r_send r2) (r_receive r1) (r_receive r2).
 
-Print _routepr_r.
- (* Definition to_action rl :=
-    match rl with
-    | route0_r => _routepr_r Ob~0~0 receive0 send0 send1
-    | route1_r => _routepr_r Ob~0~0 receive1 send0 send1
-    end. *)
+Definition routestartfn (n:nat) (r1 : reg_t): uaction reg_t empty_ext_fn_t :=
+  _routestart_r n (r_send r1) (r_receive r1). 
+
+Definition routeendfn (n:nat) (r1 : reg_t): uaction reg_t empty_ext_fn_t :=
+  _routeend_r n (r_send r1) (r_receive r1).
 
 
-
-Definition to_action rl :=
-    match rl with
-    | route0_r => _routepr_r Ob~0~0 receive0 send0 send1
-    | route1_r => _routepr_r Ob~0~0 receive1 send0 send1
-    end.
-
-  Definition schedule : scheduler :=
-  route0_r |> route1_r |> done.
-
-Print Syntax.uaction.
-
-  Definition rules :=
-    tc_rules R empty_Sigma to_action.
-
-End Design.
-
-Module PropTests.
-
-  Import Design.
-  Import Testing.
-
-  Goal
-    run_action r (rules route0_r)
-    (fun ctxt =>
-      let bits_r0 := ctxt.[ou0] in
-      Bits.to_nat bits_r0 = 49
-    ).
-  Proof.
-    check.
-  Defined.
-
-Goal
-run_action r (rules route1_r)
-    (fun ctxt =>
-      let bits_r0 := ctxt.[ou1] in
-      Bits.to_nat bits_r0 = 20
-    ).
-    Proof.
-    check.
-  Defined.
-
-
-  Goal
-    run_schedule r rules empty_sigma schedule
-    (fun ctxt =>
-       let r' := (fun idx => 
-                    match idx with
-                    | in0 => ctxt.[in0]
-                    | in1 =>  ctxt.[in1]
-                    | in0nd =>  ctxt.[in0nd]
-                    | in1nd => ctxt.[in1nd]
-                    | ou0 =>  ctxt.[ou0]
-                    | ou1 =>  ctxt.[ou1]
-                    end ) in
-
-       run_schedule r' rules empty_sigma schedule
-         (fun ctxt2 =>
-            let bits_ou0 := ctxt2.[ou0]           in
-            let nat_ou0  := Bits.to_nat bits_ou0 in
-
-            nat_ou0 = 8
-    )).
-  Proof.
-    check.
-  Defined.
-
-End PropTests.
+End Router.
