noc/NOCSyntax.v
@@ -1,0 +1,243 @@
+Require Import MetaCoq.Template.All.
+
+
+Module Type NOC_data.
+  Parameter nocsize: nat.
+End NOC_data.
+
+Module NOCSyntax (ND:NOC_data).
+Import ND.
+Import MCMonadNotation.
+Require Import List.
+From MetaCoq Require Import bytestring.
+Open Scope bs.
+(* Definition nocsize :=4. *)
+Definition regno := (Nat.sub nocsize 1).
+Definition regprefix := "r".
+Definition ruleprefix := "router_".
+
+Fixpoint rev {A : Type} (l:list A) : list A :=
+    match l with
+      | nil => nil
+      | x :: l' => rev l' ++ x :: nil
+    end.
+
+Fixpoint generate_constructors (prefix: string) (n : nat) : list constructor_body :=
+  match n with
+  | 0 => []
+  | S n' =>
+    let name := prefix ++ string_of_nat (S n') in
+    let cstr := {| cstr_name := name;
+                   cstr_args := [];
+                   cstr_indices := [];
+                   cstr_type := tRel 0;
+                   cstr_arity := 0 |} in
+    cstr :: generate_constructors prefix n'
+  end.
+
+
+Definition quoteind (ind_name : string) (prefix : string) (no_cstr :nat) :=  {|
+ind_finite := Finite;
+ind_npars := 0;
+ind_params := [];
+ind_bodies :=
+[{|
+     ind_name := ind_name;
+     ind_indices := [];
+     ind_sort := sType (Universe.make' Level.lzero);
+     ind_type := tSort (sType (Universe.make' Level.lzero));
+     ind_kelim := IntoAny;
+     ind_ctors := rev (generate_constructors prefix no_cstr);
+     ind_projs := [];
+     ind_relevance := Relevant
+   |}];
+ind_universes := Monomorphic_ctx;
+ind_variance := None
+|}.
+
+Fixpoint nat_to_term (n : nat) : term :=
+  match n with
+  | 0 => tConstruct
+          {|
+            inductive_mind :=
+              (MPfile ["Datatypes"%bs; "Init"%bs; "Coq"%bs], "nat"%bs);
+            inductive_ind := 0
+          |} 0 []
+  | S n' => tApp
+        (tConstruct
+          {|
+            inductive_mind :=
+              (MPfile ["Datatypes"%bs; "Init"%bs; "Coq"%bs], "nat"%bs);
+            inductive_ind := 0
+          |} 1 []) [nat_to_term n']
+  end.
+
+  Fixpoint generate_branches (n:nat): list (branch term) :=
+    match n with
+    | 0 => []
+    | 1 => let branchterm := {|
+          bcontext := [];
+          bbody :=
+            tApp
+              (tConst
+                (MPdot (MPfile ["Pipeline_NOC_parametric"%bs]) "Design"%bs,
+                  "routestartfn"%bs) [])
+              [(nat_to_term 0);
+              tConstruct
+                {|
+                  inductive_mind :=
+                    (MPdot (MPfile ["Pipeline_NOC_parametric"%bs])
+                        "Registers"%bs, "reg_t"%bs);
+                  inductive_ind := 0
+                |} 0 []]|} in
+    [branchterm]
+    | S n' => let branchterm := {|
+    bcontext := [];
+    bbody :=
+      tApp
+        (tConst
+           (MPdot (MPfile ["Pipeline_NOC_parametric"%bs]) "Design"%bs,
+            "routecenterfn"%bs) [])
+        [ (nat_to_term n');
+         tConstruct
+           {|
+             inductive_mind :=
+               (MPdot (MPfile ["Pipeline_NOC_parametric"%bs])
+                  "Registers"%bs, "reg_t"%bs);
+             inductive_ind := 0
+           |} (Nat.sub n' 1) [];
+         tConstruct
+           {|
+             inductive_mind :=
+               (MPdot (MPfile ["Pipeline_NOC_parametric"%bs])
+                  "Registers"%bs, "reg_t"%bs);
+             inductive_ind := 0
+           |} n' []]
+  |} in
+  branchterm :: generate_branches n'
+    end.
+  
+  
+  Definition add_last_router (l : list (branch term)) : list (branch term) :=
+    match l with
+    | [] => []
+    | _ =>
+    let last_term := {|
+    bcontext := [];
+    bbody :=
+      tApp
+        (tConst
+          (MPdot (MPfile ["Pipeline_NOC_parametric"%bs]) "Design"%bs,
+            "routeendfn"%bs) [])
+        [(nat_to_term (Nat.sub nocsize 1));
+        tConstruct
+          {|
+            inductive_mind :=
+              (MPdot (MPfile ["Pipeline_NOC_parametric"%bs])
+                  "Registers"%bs, "reg_t"%bs);
+            inductive_ind := 0
+          |} (Nat.sub nocsize 2) []]
+  |} in
+    l ++ [last_term]
+    end.
+
+Definition branch_body := Eval compute in add_last_router(rev(generate_branches regno)).
+
+Definition match_syn := (tLambda {| binder_name := nNamed "rl"%bs; binder_relevance := Relevant |}
+(tInd
+ {|
+     inductive_mind :=
+       (MPdot (MPfile ["Pipeline_NOC_parametric"%bs]) "Registers"%bs,
+        "rule_name_t"%bs);
+     inductive_ind := 0
+   |} [])
+(tCase
+   {|
+     ci_ind :=
+       {|
+         inductive_mind :=
+           (MPdot (MPfile ["Pipeline_NOC_parametric"%bs]) "Registers"%bs,
+            "rule_name_t"%bs);
+         inductive_ind := 0
+       |};
+     ci_npar := 0;
+     ci_relevance := Relevant
+   |}
+   {|
+     puinst := [];
+     pparams := [];
+     pcontext :=
+       [{| binder_name := nNamed "rl"%bs; binder_relevance := Relevant |}];
+     preturn :=
+       tApp
+         (tInd
+            {|
+              inductive_mind :=
+                (MPfile ["Syntax"%bs; "Koika"%bs], "uaction"%bs);
+              inductive_ind := 0
+            |} [])
+         [tConst (MPfile ["Frontend"%bs; "Koika"%bs], "pos_t"%bs) [];
+          tConst (MPfile ["Frontend"%bs; "Koika"%bs], "var_t"%bs) [];
+          tConst (MPfile ["Frontend"%bs; "Koika"%bs], "fn_name_t"%bs) [];
+          tInd
+            {|
+              inductive_mind :=
+                (MPdot (MPfile ["Pipeline_NOC_parametric"%bs])
+                   "Registers"%bs, "reg_t"%bs);
+              inductive_ind := 0
+            |} [];
+          tInd
+            {|
+              inductive_mind :=
+                (MPfile ["Interop"%bs; "Koika"%bs], "empty_ext_fn_t"%bs);
+              inductive_ind := 0
+            |} []]
+   |} (tRel 0)
+     branch_body
+     )).
+
+Fixpoint generate_scheduler (n: nat) : term :=
+  match n with
+  | 0 => let sterm:= tApp
+  (tConstruct
+     {|
+       inductive_mind :=
+         (MPfile ["Syntax"%bs; "Koika"%bs], "scheduler"%bs);
+       inductive_ind := 0
+     |} 0 []) 
+  [tConst (MPfile ["Frontend"%bs; "Koika"%bs], "pos_t"%bs) [];
+  tInd
+    {|
+      inductive_mind :=
+        (MPdot (MPfile ["Pipeline_NOC_parametric"%bs])
+           "Registers"%bs, "rule_name_t"%bs);
+      inductive_ind := 0
+    |} []] in sterm
+    | S n' => let sterm:= tApp (tConstruct
+    {|
+      inductive_mind :=
+        (MPfile ["Syntax"%bs; "Koika"%bs], "scheduler"%bs);
+      inductive_ind := 0
+    |} 1 [])
+    [tConst (MPfile ["Frontend"%bs; "Koika"%bs], "pos_t"%bs) [];
+    tInd
+      {|
+        inductive_mind :=
+          (MPdot (MPfile ["Pipeline_NOC_parametric"%bs])
+             "Registers"%bs, "rule_name_t"%bs);
+        inductive_ind := 0
+      |} [];
+    tConstruct
+      {|
+        inductive_mind :=
+          (MPdot (MPfile ["Pipeline_NOC_parametric"%bs])
+             "Registers"%bs, "rule_name_t"%bs);
+        inductive_ind := 0
+      |} n' []; generate_scheduler n' ]
+      in sterm
+      end.
+
+Definition scheduler_synatx := Eval compute in (generate_scheduler nocsize).
+
+End NOCSyntax.
+
