noc/Types.v
@@ -1,0 +1,33 @@
+Require Import Koika.Frontend.
+Require Import Koika.Std.
+Require Import Koika.Testing.
+
+Module Types.
+
+Definition sz := 14.
+
+Definition basic_flit :=
+    {|
+    struct_name := "basic_flit";
+    struct_fields :=
+      [
+        ("new", bits_t 1);
+        ("src" , bits_t 4);
+        ("trg_y" , bits_t 2);
+        ("trg_x" , bits_t 2);
+        ("data" , bits_t 5)
+      ]
+    |}.
+  
+Definition router_address :=
+    {|
+    struct_name := "router_address";
+    struct_fields :=
+      [
+        ("y" , bits_t 2);
+        ("x" , bits_t 2)
+      ]
+    |}.
+
+
+End Types.
